coq/proof/SimulationModule.v
@@ -373,7 +373,8 @@ Proof.
       { eapply init_mem_sem; eauto.
         - erewrite <- transl_products_genGlobalAndInitMem; eauto.
       }
-      { instantiate (1:= args0).
+      { clear SIM.
+        instantiate (1:= args0).
         instantiate (1:= args0).
         ss.
         assert(UNIQF: uniqFdef (fdef_intro (fheader_intro fnattrs0 typ0 id0 args1 varg0)
@@ -385,17 +386,12 @@ Proof.
           }
           { ss. }
         }
-        clear - WF4 WF INIT_LOCALS UNIQF.
+        unfold get_params in *.
+        exploit FIT_ARGS.
+        { ss. des_ifs. }
+        clear FIT_ARGS. intro FIT_ARGS; des.
+        clear - WF4 WF INIT_LOCALS UNIQF FIT_ARGS.
         (* initLocals_type_spec  *)
-        assert(FITGV: Forall2 (fun x y => (fit_gv (l_tgt, ndts_tgt) x.(fst).(fst) y = Some y)) args1 args0).
-        { admit. }
-        (* assert(WF_FDEF: wf_fdef [module_intro l_tgt ndts_tgt prods_src] *)
-        (*                    (module_intro l_tgt ndts_tgt prods_src) *)
-        (*                    (fdef_intro (fheader_intro fnattrs0 typ0 id0 args1 varg0) b1)). *)
-        (* { admit. } *)
-        (* inv WF_FDEF. ss. des_ifs. *)
-        (* clear H5 H9 H8. *)
-        (* inv H6. *)
         assert(NODUP: NoDup (getArgsIDs args1)).
         { inv UNIQF. ss.
           repeat match goal with
@@ -405,11 +401,11 @@ Proof.
         } clear UNIQF.
         assert(forall arg (IN: In arg args0), exists id, In id (getArgsIDs args1) /\
                                                          lookupAL GenericValue g1 id = Some arg).
-        { clear - NODUP INIT_LOCALS FITGV.
+        { clear - NODUP INIT_LOCALS FIT_ARGS.
           unfold initLocals in *.
           i.
           ginduction args0; ii; ss.
-          inv FITGV. ss. des_ifs.
+          inv FIT_ARGS. ss. des_ifs.
           des.
           - clarify. ss.
             exists i0.
@@ -434,103 +430,6 @@ Proof.
           eapply WF4; eauto.
         }
 
-(* (* NoDup (getArgsIDs la2) -> *) *)
-(* (* wf_fheader s (los, nts) (fheader_intro fattr ft fid la2 va) -> *) *)
-
-(*         assert(Forall (memory_props.MemProps.valid_ptrs (Mem.nextblock m0)) args0). *)
-(*         { *)
-(*           (* OpsemPP.initLocals_spec' *) *)
-(*           (* opsem_props.OpsemProps.initLocals_spec *) *)
-(*           clear SRC_INIT_SUCCESS. clear_tac. *)
-(*           (* OpsemPP.initializeFrameValues__wf_lc *) *)
-(*           (* gv_inject_initialize_frames *) *)
-(*           assert(Forall (fun x => lookupAl GenericValue g1  *)
-(*           unfold initLocals in *. *)
-(*           ginduction args1; ii; ss. *)
-(*           { inv H; ss. } *)
-(*           { des_ifs. inv H. ss. *)
-(*             exploit IHargs1; eauto. *)
-(*             admit. *)
-(*           } *)
-(*           ginduction args0; ii; ss. *)
-(*           { destruct args1; ss. *)
-(*             unfold initLocals in *. ss. des_ifs. *)
-(*             exploit IHargs0; eauto. *)
-(*           } *)
-(*           econs; eauto. *)
-(*         } *)
-
-
-(*         (* OpsemPP.wf_ExecutionContext__at_beginning_of_function *) *)
-(*         assert(Forall (memory_props.MemProps.valid_ptrs (Mem.nextblock m0)) args0). *)
-(*         { *)
-(*           (* OpsemPP.initLocals_spec' *) *)
-(*           (* opsem_props.OpsemProps.initLocals_spec *) *)
-
-(*           clear SRC_INIT_SUCCESS. *)
-(*           (* This is not true, I prove false below *) *)
-(*           generalize dependent args0. *)
-(*           generalize dependent args1. *)
-(*           generalize dependent g1. *)
-(*           assert(~forall g1 : GVsMap, *)
-(*                       memory_props.MemProps.wf_lc m0 g1 -> *)
-(*                       (forall (i0 : atom) (gv : GenericValue), *)
-(*                           lookupAL GenericValue g1 i0 = ret gv -> *)
-(*                           genericvalues_inject.gv_inject (memory_props.MemProps.inject_init *)
-(*                                                             (Mem.nextblock m0 - 1)) gv gv) -> *)
-(*                       forall (args1 : args) (args0 : list GenericValue), *)
-(*                         initLocals (l_tgt, ndts_tgt) args1 args0 = ret g1 -> *)
-(*                         Forall (memory_props.MemProps.valid_ptrs (Mem.nextblock m0)) args0). *)
-(*           { ii. *)
-(*             specialize (H []). *)
-(*             exploit H. *)
-(*             { ss. } *)
-(*             { ii. ss. } *)
-(*             { instantiate (1:= [[((Vptr (m0.(Mem.nextblock)) (Int.repr 31 0)), AST.Mfloat32)]]). *)
-(*               instantiate (1:= []). *)
-(*               ss. *)
-(*             } *)
-(*             i. inv x. inv H2. eapply Plt_irrefl; eauto. *)
-(*           } *)
-(*           admit. *)
-(*         } *)
-(*         clear - H. *)
-(*         ginduction args0; ii; ss. *)
-(*         - econs; eauto. *)
-(*         - inv H. econs; eauto. *)
-(*           clear - H2. *)
-(*           ginduction a; ii; ss. *)
-(*           des_ifs; ss; try (by econs; eauto). *)
-(*           des. *)
-(*           unfold memory_props.MemProps.inject_init. *)
-(*           econs; eauto. *)
-(*           econs; eauto. *)
-(*           { des_ifs. exfalso. *)
-(*             rewrite Pos.leb_nle in Heq. apply Heq. *)
-(*             rewrite <- Pos.lt_succ_r. *)
-(*             abstr (Mem.nextblock m0) a. *)
-(*             clear - H2. *)
-(*             eapply Pos.lt_le_trans; eauto. clear - a. *)
-(*             rewrite <- Pos.add_1_r. *)
-(*             destruct a eqn:T; ss. *)
-(*             - reflexivity. *)
-(*             - rewrite Pos.sub_add. *)
-(*               + reflexivity. *)
-(*               + destruct b; ss. *)
-(*           } *)
-(*           { clear - i0. *)
-(*             destruct i0; ss. *)
-(*             unfold Int.add; ss. *)
-(*             rewrite Z.add_0_r. *)
-(*             unfold Int.repr. *)
-(*             apply Int.mkint_eq; eauto. *)
-(*             rewrite Int.Z_mod_modulus_eq. *)
-(*             abstr (Int.modulus 31) X. *)
-(*             des. *)
-(*             rewrite Zdiv.Zmod_small; ss. *)
-(*             omega. *)
-(*           } *)
-(*       } *)
       { econs; ss; eauto. }
       clear SIM. intro SIM_LOCAL; des.
       inv SIM_LOCAL. ss. clarify.
@@ -555,4 +454,7 @@ Proof.
             split; ss.
           }
         * reflexivity.
-Admitted.
+  }
+Unshelve.
+all: try (by ss).
+Qed.
